src/Helpers/Integers.v
@@ -1,0 +1,41 @@
+From Coq Require Export BinNat.
+
+From stdpp Require Import decidable countable.
+From bbv Require Import Word.
+
+Open Scope N_scope.
+
+(* this is sort of a big number *)
+Definition n64: nat := 64.
+Notation u64 := (word n64).
+Definition u64_max : N := Npow2 n64.
+Opaque u64_max.
+
+Instance word_eq_dec sz : EqDecision (word sz) := @weq sz.
+Instance word_countable sz : Countable (word sz).
+Proof.
+  apply (inj_countable
+           (@wordToN sz)
+           (fun n => Some (NToWord sz n))); intros.
+  by rewrite NToWord_wordToN.
+Qed.
+
+Instance wlt_decide sz : Decision (@wlt sz x y) := @wlt_dec sz.
+
+(* TODO: note that these wrappers are inconvenient so we're actually using word
+functions directly; if the indirection is useful we can add it and make u64
+opaque *)
+
+Definition add_u64 : u64 -> u64 -> u64 := @wplus _.
+Definition minus_u64 : u64 -> u64 -> u64 := @wminus _.
+Definition mult_u64 : u64 -> u64 -> u64 := @wmult _.
+
+Definition u64_v : u64 -> N := @wordToN _.
+
+Theorem u64_bound : forall (x:u64), u64_v x < u64_max.
+Proof.
+  intros.
+  apply wordToN_bound.
+Qed.
+
+Definition byte := (word 8).
